

① $Y = X + Z$

$$f_X(x) = f_Z(x) = \frac{1}{\sqrt{2\pi \times 4}} e^{-\frac{1}{2} \left(\frac{x-2}{2} \right)^2}$$

② $f_{X,Y}(x,y) = f_{X,Z}(x, y-x)$

$$\begin{aligned} (x,y) &\Leftrightarrow (x,z) \\ x &= z \\ Y &= X + Z \end{aligned} \quad \begin{aligned} &= f_X(x) f_Z(y-x) \\ &= f_X(x) f_{Y|X}(y|x) \end{aligned}$$

\Rightarrow $f_{Y|X}(y|x) = f_Z(y-x)$ ↖ mark

$$f_Y(y) = \int_{-\infty}^{\infty} f_X(x) f_{Y|X}(y|x) dx$$

$$= \int_{-\infty}^{\infty} f_X(x) f_Z(y-x) dx$$

$\mu=2$
 $\sigma=2$

$$= \int_{-\infty}^{\infty} \frac{1}{(\sqrt{2\pi}\sigma)^2} e^{-\frac{1}{2} \left(\frac{x-\mu}{\sigma} \right)^2} e^{-\frac{1}{2} \left(\frac{y-x-\mu}{\sigma} \right)^2} dx$$

$$= \int_{-\infty}^{\infty} \frac{1}{(\sqrt{2\pi}\sigma)^2} e^{-\frac{1}{2} \left[\left(\frac{x-\mu}{\sigma} \right)^2 + \left(\frac{y-x-\mu}{\sigma} \right)^2 - 2 \frac{(x-\mu)(y-x-\mu)}{\sigma^2} \right]} dx$$

$$= \int_{-\infty}^{\infty} \frac{1}{(\sqrt{2\pi}\sigma)^2} e^{-\frac{1}{2} \left[\left(\frac{x-\mu}{\sigma} \right)^2 - 2 \frac{\sqrt{2}}{\sigma} \left(\frac{x-\mu}{\sigma} \right) \left(\frac{y-2\mu}{\sqrt{2}\sigma} \right) + \left(\frac{y-2\mu}{\sqrt{2}\sigma} \right)^2 + \left(\frac{y-2\mu}{\sqrt{2}\sigma} \right)^2 \right]} dx$$

$$= \frac{e^{-\left(\frac{y-2\mu}{\sqrt{2}\sigma} \right)^2}}{\sqrt{2\pi}\sigma\sqrt{2}} \int_{-\infty}^{\infty} \frac{\sqrt{2}}{\sqrt{2\pi}\sigma} e^{-\frac{1}{2(\sigma^2/2)} \left[(x-\mu) - \left(\frac{y-2\mu}{2} \right) \right]^2} dx$$

density of

$$N\left(\frac{y}{2}, \sigma^2/2\right).$$

\therefore should sum to 1.

$$= \frac{e^{-\left(\frac{y-2\mu}{\sqrt{2}\sigma} \right)^2}}{\sqrt{2\pi}\sigma\sqrt{2}}$$

Please give them marks if they assumed Sum of Gaussian is Gaussian.

$$E[Y] = E[X] + E[Z] = 4,$$

$$\text{Var}(Y) = \text{Var}(X) + \text{Var}(Z) = 8$$

$$\Rightarrow Y \sim N(4, 8)$$

$$\Rightarrow f_Y(y) = \frac{1}{\sqrt{2\pi \times 8}} e^{-\frac{1}{2} \frac{(y-4)^2}{8}}$$

\rightarrow ① mark

$$f_{X|Y}(x|y) = \frac{f_X(x) f_{Y|X}(y|x)}{f_Y(y)}.$$

0.5

$$= \frac{\frac{1}{\sqrt{2\pi}\sigma^2} e^{-\frac{1}{2}\left(\frac{x-\mu}{\sigma}\right)^2}}{\frac{1}{\sqrt{2\pi}\sigma^2 \times 2} e^{-\frac{1}{2}\left(\frac{y-2\mu}{\sqrt{2}\sigma}\right)^2}}$$

$$0.5 \leftarrow = \frac{1}{\sqrt{2\pi}(\sigma/\sqrt{2})} e^{-\frac{1}{2} \frac{(x-y/2)^2}{(\sigma^2/2)}}$$

(b) MMSE estimator . $\hat{x}_{\text{MMSE}}[y] = E[x|Y=y]$ (1.5)

$E[x|Y] = y/2$ as (1.5) $X|Y=y$ is $N(y/2, \sigma^2/2)$.

(c) MAP estimator .

$$\hat{x}_{\text{MAP}}(y) = \arg \max_x f_{X|Y}(x|y) = \arg \max_x e^{-\frac{1}{2}\left(\frac{x-y/2}{\sigma/\sqrt{2}}\right)^2}$$

1 \leftarrow = $y/2$

$$\Rightarrow \hat{x}_{\text{MAP}}(y) = y/2$$

ML estimator

$$\hat{x}_{\text{ML}}(y) = \arg \max_x f_{Y|X}(y|x) = \arg \max_x f_Z(y-x)$$

1 \leftarrow = $\arg \max_x e^{-\frac{1}{2}\left(\frac{y-x-\mu}{\sigma}\right)^2}$

$$= y - \mu.$$

$$\Rightarrow \hat{x}_{ML}(y) = y - \mu = y - 2.$$

$$\textcircled{d} \quad \text{Var}(Y) = \text{Var}(X) + \text{Var}(Z) = 8 \rightarrow \textcircled{1}$$

$$E[Y] = E[X] + E[Z] = 4 \rightarrow \textcircled{1}$$

$$\text{Cov}(X, Y) = E[X Y] - E[X] E[Y]$$

$$E[X Y] = E[X(X+Z)]$$

$$= E[X^2 + XZ]$$

$$= E[X^2] + E[X] E[Z]$$

$$= (4+4) + 2 \times 2.$$

$$= 12.$$

$$\text{Cov}(X, Y) = 12 - 2 \times 4 = 4 \rightarrow \textcircled{2}$$

$$\textcircled{e} \quad \hat{x}_{LMMSE}(y) = \frac{\text{Cov}(X, Y)}{\text{Var}(Y)} (y - E[Y]) + E[X].$$

$$= \frac{4}{8} (y - 4) + 2.$$

$$\textcircled{1} \leftarrow = y/2.$$

give marks
even if
there are
calculation
mistakes

⑦

$$E \left[\left(X - \hat{x}_{\text{LMMSE}}(Y) \right)^2 \right] = E \left[\left(X - \frac{Y}{2} \right)^2 \right]$$

0.5 for writing this expression

$$= \text{Var}(X) - \frac{\text{Cov}(X, Y)^2}{\text{Var}(Y)}$$

1.5

$$= 4 - \frac{4^2}{8} = 2$$

$$= E \left[\left(X - \frac{X+Z}{2} \right)^2 \right]$$

$$= \frac{1}{4} E \left[(X-Z)^2 \right]$$

$$= \frac{1}{4} [8 + 8 - 2 \times 2 \times 2] = 2$$

⑧

should have same error for LMMSE, MAP, MMSE estimator are all the same in this case: as these three estimators are the same.

3 marks

ML error

$$E \left[\left(X - \hat{x}_{\text{ML}}(Y) \right)^2 \right]$$

0.5

$$= E \left[\left(X - (Y-2) \right)^2 \right]$$

$$= E \left[X^2 + (Y-2)^2 - 2X(Y-2) \right]$$

$$= E[X^2] + E[(Y-2)^2] - 2E[X(Y-2)]$$

$$= \text{Var}(X) + (E[X])^2 + \text{Var}(Y-2) + (E[Y-2])^2 - 2E[XY] + 4E[X]$$

2.5

$$= 4 + (2)^2 + 8 + (2)^2 - 2 \times 12 + 4 \times 2$$

$$\text{Var}(Y-2) = \text{Var}(Y)$$

$$E[Y-2] = E[Y] - 2$$

give partial
marks for
intermediate
steps.

= 4.